started InsertionSort

TP3/InsertionSort.dfy
@@ -1,15 +1,43 @@
+predicate isSorted(a: array<int>)
+    reads a
+{
+    forall i, j :: 0 <= i < j < a.Length ==> a[i] <= a[j]
+}
+
+predicate isSortedSub(a: array<int>, left: nat, right: nat)
+    reads a
+    requires 0 <= left <= right < a.Length
+{
+    forall i, j :: left <= i < j < right ==> a[i] <= a[j]
+}
+
+
 // Sorts array 'a' using the insertion sort algorithm.
 method insertionSort(a: array<int>)
+  modifies a
+
+  requires a.Length > 0
+
+  ensures isSorted(a)
+  ensures multiset(a[..]) == multiset(old(a[..]))
 {
     var i := 0;
     while i < a.Length 
-    {
+      decreases  a.Length - i
+      invariant 0 <= i < a.Length
+      invariant multiset(a[..]) == multiset(old(a[..]))
+  {
         var j := i;
         while j > 0 && a[j-1] > a[j]
+          decreases j
+          invariant 0 < j <= i
+          invariant isSortedSub(a, j, i + 1)
+          invariant multiset(a[..]) == multiset(old(a[..]))
         {
             a[j-1], a[j] := a[j], a[j-1];
             j := j - 1;
         }
+        
         i := i + 1;
     }
 }
